Reap/Test/Tactic/MCTS.lean
@@ -1,6 +1,21 @@
 import Reap.Tactic.Syntax
 
+open Reap.TreeSearch
+
 set_option linter.unusedSimpArgs false
+
+def andOrTacGen : TacGen := fun _ => do
+  return #[
+    ("constructor", #[], 1.0),
+    ("exact hP", #[], 1.0),
+    ("exact hQ", #[], 1.0)
+  ]
+
+def andOrStateEval : StateEval := fun _ => do
+  return 0.0
 
 example : (a b c : Nat) → a = b → b = c → a = c := by
   reapMCTS
+
+example (P Q : Prop) (hP : P) (hQ : Q) : P ∧ Q := by
+  run_tac reapMCTS andOrTacGen andOrStateEval (maxNodes := 32) (maxSteps := 32)
